crypto_examples/mulntt_ct/intt_ct.dfy
@@ -1,0 +1,124 @@
+include "intt_rec.dfy"
+
+abstract module intt_ct {
+    import opened Seq
+    import opened Power
+    import opened Power2
+    import opened DivMod
+    import opened Mul
+
+    import opened pows_of_2
+    import opened nth_root
+    import opened ntt_index
+
+    import opened innt_model
+    import opened ntt_polys
+
+    method j_loop(a: n_sized, p: n_sized, t: pow2_t, d: pow2_t, j: nat, ghost view: intt_loop_view)
+    returns (a': n_sized)
+        requires view.j_loop_inv(a, d, j);
+        requires t == view.lsize();
+        requires p == rev_omega_inv_powers_mont_table();
+        requires j < view.lsize().full;
+        ensures view.j_loop_inv(a', d, j + 1);
+    {
+        view.s_loop_inv_pre_lemma(a, d, j);
+
+        var u := (2 * j) * d.full;
+        rev_omega_inv_powers_mont_table_lemma(t, d, j);
+        var w := p[t.full + j];
+
+        var s := u;
+        a' := a;
+
+        ghost var bi := 0;
+
+        while (s < u + d.full)
+            invariant view.s_loop_inv(a', d, j, s-u);
+        {
+            var a :n_sized := a';
+            var bi := s-u;
+
+            var _ := view.higher_points_view_index_lemma(a, d, j, bi);
+
+            var e := a[s];
+            var o := a[s + d.full];
+
+            var x := montmul(o, w);
+            a' := a[s+d.full := mqsub(e, x)];
+            a' := a'[s := mqadd(e, x)];
+            s := s + 1;
+
+            view.s_loop_inv_peri_lemma(a, a', d, j, bi);
+        }
+
+        assert s == u + d.full;
+        view.s_loop_inv_post_lemma(a', d, j, d.full);
+    }
+
+    method t_loop(a: n_sized, p: n_sized, t: pow2_t, d: pow2_t, ghost view: intt_loop_view)
+        returns (a': n_sized, ghost view': intt_loop_view)
+
+        requires view.t_loop_inv(a, d);
+        requires p == rev_omega_inv_powers_mont_table();
+        requires t == view.lsize();
+        requires t.exp < N.exp;
+
+        ensures view.hsize.exp < N.exp ==> view'.t_loop_inv(a', pow2_half(d));
+        ensures view.hsize.exp == N.exp ==> view' == view;
+        ensures view.hsize.exp == N.exp ==> view'.t_loop_end(a');
+    {
+        var j := 0;
+        a' := a;
+
+        view.j_loop_inv_pre_lemma(a', d);
+
+        while (j < t.full)
+            invariant t == view.lsize();
+            invariant view.j_loop_inv(a', d, j);
+        {
+            a' := j_loop(a', p, t, d, j, view);
+            j := j + 1;
+        }
+
+        view' := view.j_loop_inv_post_lemma(a', d, j);
+    }
+
+    method mulntt_ct(a: n_sized, p: n_sized, ghost view: intt_loop_view)
+        returns (a': n_sized, ghost view': intt_loop_view)
+        requires N.exp >= 1;
+        requires view.t_loop_inv(a, pow2(N.exp-1));
+        requires p == rev_omega_inv_powers_mont_table();
+        ensures view'.t_loop_end(a');
+    {
+        var d := pow2(N.exp);
+        var t := pow2(0);
+        a' := a;
+        view' := view;
+
+        assert view'.lsize() == pow2(0) by {
+            view'.size_count_lemma();
+        }
+
+        pow2_basics(t);
+
+        Nth_root_lemma();
+
+        while (t.full < N.full)
+            invariant 1 <= d.exp <= N.exp;
+            invariant view'.t_loop_inv(a', pow2_half(d));
+            invariant t.full >= N.full ==> view'.hsize.exp == N.exp;
+            invariant t == view'.lsize();
+        {
+            d := pow2_half(d);
+            a', view' := t_loop(a', p, t, d, view');
+            t := pow2_double(t);
+
+            if t.full >= N.full {
+                assume view'.hsize.exp == N.exp;
+            }
+        }
+
+        assert view'.hsize.exp == N.exp;
+    }
+}
