crypto_examples/mulntt_ct/intt_rec.dfy
@@ -1,0 +1,984 @@
+include "../mulntt_ct/nth_root.dfy"
+
+abstract module innt_model {
+    import opened Seq
+    import opened Power
+    import opened Power2
+    import opened DivMod
+    import opened Mul
+
+	import opened pows_of_2
+    import opened ntt_index
+    import opened nth_root
+    import opened ntt_polys
+
+    const x_value: x_fun := rev_omega_inv_powers_x_value;
+
+    datatype intt_loop_view = intt_loop_view(
+        lower: seq<seq<elem>>, // lower polys
+        higher: seq<seq<elem>>, // higher polys
+        hsize: pow2_t)
+    {
+        predicate loop_view_wf()
+        {
+            && 1 <= hsize.exp <= N.exp
+            && unifromly_sized(higher, hsize)
+            && build_lower_level(higher, hsize) == lower
+        }
+
+        function lsize(): pow2_t
+            requires loop_view_wf();
+        {
+            pow2_half(hsize)
+        }
+
+        function lcount(): pow2_t
+            requires loop_view_wf();
+        {
+            block_count(lsize())
+        }
+
+        function hcount(): pow2_t
+            requires loop_view_wf();
+        {
+            block_count(hsize)
+        }
+
+        // a very boring lemma 
+        lemma size_count_lemma()
+            requires loop_view_wf();
+            ensures pow2_double(lsize()) == hsize;
+            ensures lcount() == pow2_double(hcount());
+            ensures N.full
+                == lcount().full * lsize().full
+                == lsize().full * lcount().full 
+                == hcount().full * hsize.full
+                == hsize.full * hcount().full;
+            ensures pow2_half(N).full
+                == lsize().full * hcount().full
+        {
+            Nth_root_lemma();
+            block_count_half_lemma(hsize);
+            LemmaMulIsCommutative(lcount().full, lsize().full);
+            LemmaMulIsCommutative(hsize.full, hcount().full);
+            block_count_half_lemma(lcount());
+
+            LemmaMulIsAssociative(2, lsize().full, hcount().full);
+            assert 2 * lsize().full * hcount().full == N.full;
+            LemmaFundamentalDivModConverse(N.full, 2, lsize().full * hcount().full, 0);
+        }
+
+        predicate {:opaque} t_loop_low_inv(a: n_sized, hcount: pow2_t)
+            requires hcount.exp < N.exp;
+            requires loop_view_wf();
+            requires hsize == block_size(hcount);
+        {
+            && var lcount := lcount();
+            && var lpoints := level_points_view(a, lsize());
+            && (forall i | 0 <= i < lcount.full ::
+                points_eval_inv(lpoints[i], lower[bit_rev_int(i, lcount)], x_value, lcount))
+        }
+
+        predicate t_loop_inv(a: n_sized, hcount: pow2_t)
+        {
+            && loop_view_wf()
+            && 0 <= hcount.exp < N.exp
+            && hsize == block_size(hcount)
+            && t_loop_low_inv(a, hcount)
+        }
+
+        // static function init_loop_view(): (v: loop_view) 
+        //     ensures v.loop_view_wf();
+        // {   
+        //     var hsize := pow2(1);
+        //     loop_view(
+        //         level_polys(pow2_half(hsize)), 
+        //         level_polys(hsize),
+        //         hsize)
+        // }
+
+        // lemma init_loop_view_lemma(a: n_sized)
+        //     requires this == init_loop_view();
+        // {
+        //     pow2_basics(hsize);
+        //     size_count_lemma();
+        //     assert lsize() == pow2(0);
+        //     var lcount := lcount();
+        //     var lpoints := level_points_view(a, lsize());
+        //     var hcount := hcount();
+
+        //     Nth_root_lemma();
+        //     assert lcount == pow2(N.exp); 
+        //     assert hcount == pow2(N.exp-1);
+
+        //     assert t_loop_low_inv(a, hcount) by {
+        //         forall i | 0 <= i < lcount.full
+        //             ensures points_eval_inv(lpoints[i], lower[bit_rev_int(i, lcount)], lcount);
+        //         {
+        //             assume false;
+        //         }
+        //         reveal t_loop_low_inv(); 
+        //     }
+        // }
+
+        predicate t_loop_end(a: n_sized)
+        {
+            && loop_view_wf()
+            && hsize.exp == N.exp
+            && var hpoints := level_points_view(a, hsize);
+            && |hpoints| == 1
+            && |higher| == 1
+            && points_eval_inv(hpoints[0], higher[0], x_value, pow2(0))
+        }
+
+        lemma x_value_even_square_lemma(j: nat, x: elem)
+            requires loop_view_wf();
+            requires 2 * j < hsize.full;
+            requires x == x_value(2 * j, hcount());
+            ensures mqmul(x, x) == x_value(j, lcount());
+        {
+            size_count_lemma();
+            var hc := hcount();
+
+            LemmaMulNonnegative(bit_rev_int(2 * j, hsize), hc.full);
+            LemmaMulIsAssociative(2, bit_rev_int(2 * j, hsize), hc.full);
+            var exp := bit_rev_int(2 * j , hsize) * hc.full;
+
+            assert x == mqpow(OMEGA_INV, exp);
+
+            calc == {
+                2 * exp;
+                2 * (bit_rev_int(2 * j , hsize) * hc.full);
+                {
+                    bit_rev_int_lemma2(j, lsize());
+                }
+                2 * (bit_rev_int(j, lsize()) * hc.full);
+                {
+                    LemmaMulProperties();
+                }
+                bit_rev_int(j, lsize()) * (2 * hc.full);
+                bit_rev_int(j, lsize()) * lcount().full;
+            }
+    
+            var temp := Pow(OMEGA_INV, exp);
+    
+            calc == {
+                mqmul(x, x);
+                ((temp % Q) * (temp % Q)) % Q;
+                {
+                    LemmaMulModNoopGeneral(temp, temp, Q);
+                }
+                (temp * temp) % Q;
+                {
+                    LemmaPowAdds(OMEGA_INV, exp, exp);
+                    assert exp + exp == 2 * exp;
+                }
+                Pow(OMEGA_INV, 2 * exp) % Q;
+                x_value(j, lcount());
+            }
+        }
+
+        lemma x_value_odd_square_lemma(j: nat, x: elem)
+            requires loop_view_wf();
+            requires 2 * j < hsize.full;
+            requires x == x_value(2 * j + 1, hcount());
+            ensures mqmul(x, x) == x_value(j, lcount());
+        {
+            size_count_lemma();
+            var hc := hcount();
+
+            LemmaMulNonnegative(bit_rev_int(2 * j + 1, hsize), hc.full);
+            LemmaMulIsAssociative(2, bit_rev_int(2 * j + 1, hsize), hc.full);
+            var exp := bit_rev_int(2 * j + 1, hsize) * hc.full;   
+            assert x == mqpow(OMEGA_INV, exp);
+            var temp := Pow(OMEGA_INV, exp);
+    
+            calc == {
+                2 * exp;
+                2 * (bit_rev_int(2 * j + 1, hsize) * hc.full);
+                {
+                    LemmaMulProperties();
+                }
+                (2 * bit_rev_int(2 * j + 1, hsize)) * hc.full;
+                {
+                    bit_rev_int_lemma3(j, lsize());
+                }
+                (2 * (bit_rev_int(j, lsize()) + lsize().full)) * hc.full;
+                {
+                    LemmaMulIsDistributive(2, bit_rev_int(j, lsize()), lsize().full);
+                }
+                (2 * bit_rev_int(j, lsize()) + 2 * lsize().full) * hc.full;
+                {
+                    LemmaMulIsDistributive(hc.full, 2 * bit_rev_int(j, lsize()), 2 * lsize().full);
+                }
+                2 * bit_rev_int(j, lsize()) * hc.full + 2 * lsize().full * hc.full;
+                2 * bit_rev_int(j, lsize()) * hc.full + N.full;
+                {
+                    LemmaMulProperties();
+                }
+                bit_rev_int(j, lsize()) * (2 * hc.full) + N.full;
+                bit_rev_int(j, lsize()) * lcount().full + N.full;
+            }
+
+            calc == {
+                mqmul(x, x);
+                ((temp % Q) * (temp % Q)) % Q;
+                {
+                    LemmaMulModNoopGeneral(temp, temp, Q);
+                }
+                (temp * temp) % Q;
+                {
+                    LemmaPowAdds(OMEGA_INV, exp, exp);
+                }
+                Pow(OMEGA_INV, 2 * exp) % Q;
+                Pow(OMEGA_INV, bit_rev_int(j, lsize()) * lcount().full + N.full) % Q;
+                {
+                    LemmaMulNonnegative(bit_rev_int(j, lsize()), lcount().full);
+                    inv_full_rotation_lemma(bit_rev_int(j, lsize()) * lcount().full);
+                }
+                Pow(OMEGA_INV, bit_rev_int(j, lsize()) * lcount().full) % Q;
+            }
+        }
+
+        predicate {:opaque} j_loop_higher_inv(a: n_sized, hcount: pow2_t, j: nat)
+            requires hcount.exp <= N.exp;
+            requires loop_view_wf();
+            requires hsize == block_size(hcount);
+        {
+            && var hpoints := level_points_view(a, hsize);
+            && (forall i | 0 <= i < hcount.full ::
+                points_eval_prefix_inv(hpoints[i], higher[bit_rev_int(i, hcount)], x_value, 2*j, hcount))
+        }
+
+        predicate {:opaque} j_loop_lower_inv(a: n_sized, hcount: pow2_t, j: nat)
+            requires hcount.exp <= N.exp;
+            requires loop_view_wf();
+            requires hsize == block_size(hcount);
+        {
+            && var lcount := lcount();
+            && var lpoints := level_points_view(a, lsize());
+            && (forall i | 0 <= i < lcount.full ::
+                points_eval_suffix_inv(lpoints[i], lower[bit_rev_int(i, lcount)], x_value, j, lcount))
+        }
+
+        predicate j_loop_inv(a: n_sized, hcount: pow2_t, j: nat)
+        {
+            && loop_view_wf()
+            && hcount.exp <= N.exp
+            && hsize == block_size(hcount)
+            && j <= lsize().full
+            && j_loop_higher_inv(a, hcount, j)
+            && j_loop_lower_inv(a, hcount, j)
+        }
+
+        predicate {:opaque} s_loop_higher_inv(a: n_sized, hcount: pow2_t, j: nat, bi: nat)
+            requires hcount.exp <= N.exp;
+            requires bi <= hcount.full;
+            requires loop_view_wf();
+            requires hsize == block_size(hcount);
+        {
+            && var hpoints := level_points_view(a, hsize);
+            && (forall i | 0 <= i < bi ::
+                points_eval_prefix_inv(hpoints[i], higher[bit_rev_int(i, hcount)], x_value, 2*j+2, hcount))
+            && (forall i | bi <= i < hcount.full ::
+                points_eval_prefix_inv(hpoints[i], higher[bit_rev_int(i, hcount)], x_value, 2*j, hcount))
+        }
+
+        predicate {:opaque} s_loop_lower_inv(a: n_sized, hcount: pow2_t, j: nat, bi: nat)
+            requires hcount.exp <= N.exp;
+            requires bi <= hcount.full;
+            requires loop_view_wf();
+            requires hsize == block_size(hcount);
+        {
+            size_count_lemma();
+            && var lcount := lcount();
+            && var lpoints := level_points_view(a, lsize());
+            && (forall i | (0 <= i < bi || hcount.full <= i < bi + hcount.full) ::
+                && (points_eval_suffix_inv(lpoints[i], lower[bit_rev_int(i, lcount)], x_value, j+1, lcount)))
+            && (forall i | (bi <= i < hcount.full || bi + hcount.full <= i < lcount.full) ::
+                points_eval_suffix_inv(lpoints[i], lower[bit_rev_int(i, lcount)], x_value, j, lcount))
+        }
+
+        predicate s_loop_inv(a: n_sized, hcount: pow2_t, j: nat, bi: nat)
+        {
+            && loop_view_wf()
+            && hcount.exp <= N.exp
+            && bi <= hcount.full
+            && j < lsize().full
+            && hsize == block_size(hcount)
+            && s_loop_higher_inv(a, hcount, j, bi)
+            && s_loop_lower_inv(a, hcount, j, bi)
+        }
+
+        // lemma s_loop_index_bound(a: n_sized, hcount: pow2_t, j: nat, bi: nat)
+        //     requires loop_view_wf();
+        //     requires hcount.exp <= N.exp;
+        //     requires bi < hcount.full;
+        //     requires j < lsize().full;
+        //     requires hsize == block_size(hcount);
+        //     ensures bi + (2*j) * hcount.full + hcount.full < N.full;
+        //     ensures bi + hcount.full < lcount().full;
+        // {
+        //     size_count_lemma();
+        //     point_view_index_bound_lemma(bi, 2 * j+1, hsize);
+        //     LemmaMulIsDistributive(hcount.full, 2*j, 1);
+        //     assert (2*j) * hcount.full + hcount.full == (2*j + 1) * hcount.full;
+        // }
+
+        lemma higher_points_view_index_lemma(a: n_sized, hcount: pow2_t, j: nat, bi: nat)
+            returns (s: nat)
+    
+            requires s_loop_inv(a, hcount, j, bi);
+            requires bi < hcount.full
+            ensures s == bi + (2*j) * hcount.full;
+            ensures s + hcount.full < N.full;
+            ensures a[s] == level_points_view(a, hsize)[bi][2*j];
+            ensures s == point_view_index(bi, 2*j, hsize);
+            ensures a[s+hcount.full] == level_points_view(a, hsize)[bi][2*j+1];
+            ensures s+hcount.full == point_view_index(bi, 2*j+1, hsize);
+        {
+            size_count_lemma();
+            var hpoints := level_points_view(a, hsize);
+            LemmaMulNonnegative(2*j, hcount.full);
+            s := bi + (2*j) * hcount.full;
+
+            calc == {
+                hpoints[bi][2*j];
+                points_view(a, bi, hsize)[2*j];
+                a[point_view_index(bi, 2*j, hsize)];
+                {
+                    assert s == point_view_index(bi, 2*j, hsize);
+                }
+                a[s];
+            }
+
+            calc == {
+                s + hcount.full;
+                point_view_index(bi, 2*j, hsize) + hcount.full;
+                bi + (2*j) * hcount.full + hcount.full;
+                {
+                    LemmaMulIsDistributiveAddOtherWayAuto();
+                }
+                bi + (2*j+1) * hcount.full;
+                point_view_index(bi, 2*j+1, hsize);
+            }
+
+            calc == {
+                hpoints[bi][2*j+1];
+                points_view(a, bi, hsize)[2*j+1];
+                a[point_view_index(bi, 2*j+1, hsize)];
+                a[s + hcount.full];
+            }
+        }
+
+        lemma lower_points_view_index_lemma(a: n_sized, hcount: pow2_t, j: nat, bi: nat)
+            returns (s: nat)
+
+            requires s_loop_inv(a, hcount, j, bi);
+            requires bi < hcount.full
+            ensures s == bi + (2*j) * hcount.full;
+            ensures s + hcount.full < N.full;
+            ensures bi + hcount.full < lcount().full;
+            ensures a[s] == level_points_view(a, lsize())[bi][j];
+            ensures s == point_view_index(bi, j, lsize());
+            ensures a[s+hcount.full] == level_points_view(a, lsize())[bi+hcount.full][j];
+            ensures s+hcount.full == point_view_index(bi+hcount.full, j, lsize());
+        {
+            size_count_lemma();
+            var lpoints := level_points_view(a, lsize());
+            LemmaMulNonnegative(2*j, hcount.full);
+            s := bi + (2*j) * hcount.full;
+
+            calc == {
+                s;
+                bi + (2*j) * hcount.full;
+                {
+                    LemmaMulIsAssociativeAuto();
+                }
+                bi + j * (2*hcount.full);
+                point_view_index(bi, j, lsize());
+            }
+
+            calc == {
+                lpoints[bi][j];
+                points_view(a, bi, lsize())[j];
+                a[point_view_index(bi, j, lsize())];
+                a[s];
+            }
+
+            calc == {
+                s + hcount.full;
+                bi + hcount.full + (j*2) * hcount.full;
+                {
+                    LemmaMulIsAssociativeAuto();
+                }
+                bi + hcount.full + j * (2 * hcount.full);
+                bi + hcount.full + j * lcount().full;
+                point_view_index(bi +  hcount.full, j, lsize());
+            }
+
+            calc == {
+                lpoints[bi+hcount.full][j];
+                points_view(a, bi+hcount.full, lsize())[j];
+                a[point_view_index(bi+hcount.full, j, lsize())];
+                a[s+hcount.full];
+            }
+        }
+
+        function get_even_poly(bi: nat): seq<elem>
+            requires loop_view_wf();
+            requires bi < lcount().full;
+        {
+            lower[bit_rev_int(bi, lcount())]
+        }
+
+        function get_odd_poly(bi: nat): seq<elem>
+            requires loop_view_wf();
+            requires bi + hcount().full < lcount().full;
+        {
+            lower[bit_rev_int(bi+hcount().full, lcount())]
+        }
+
+        function get_full_poly(bi: nat): seq<elem>
+            requires loop_view_wf();
+            requires bi < hcount().full;
+        {
+            higher[bit_rev_int(bi, hcount())]
+        }
+    
+        lemma lower_points_view_value_lemma(a: n_sized, hcount: pow2_t, j: nat, bi: nat, s: nat)
+            requires s_loop_inv(a, hcount, j, bi);
+            requires bi < hcount.full
+            requires s == bi + (2*j) * hcount.full;
+            ensures s + hcount.full < N.full;
+            ensures bi + hcount.full < lcount().full;
+            ensures a[s] == poly_eval(get_even_poly(bi), x_value(j, lcount()));
+            ensures a[s+hcount.full] == poly_eval(get_odd_poly(bi), x_value(j, lcount()));
+        {
+            size_count_lemma();
+            var _ := lower_points_view_index_lemma(a, hcount, j, bi);
+            var lpoints := level_points_view(a, lsize());
+            var lcount := lcount();
+
+            var e_poly := get_even_poly(bi);
+            var e_points := lpoints[bi];
+
+            assert a[s] == poly_eval(e_poly, x_value(j, lcount)) by {
+                assert points_eval_suffix_inv(e_points, e_poly, x_value, j, lcount) by {
+                    reveal s_loop_lower_inv();
+                }
+                reveal points_eval_suffix_inv();
+                assert a[s] == e_points[j];
+            }
+
+            var o_poly := get_odd_poly(bi);
+            var o_points := lpoints[bi+hcount.full];
+
+            assert a[s+hcount.full] == poly_eval(o_poly, x_value(j, lcount)) by {
+                assert points_eval_suffix_inv(o_points, o_poly, x_value, j, lcount) by {
+                    reveal s_loop_lower_inv();
+                }
+                reveal points_eval_suffix_inv();
+                assert a[s+hcount.full] == lpoints[bi+hcount.full][j];
+            }
+        }
+
+        lemma level_polys_bitrev_index_correspondence_lemma(a: n_sized, hcount: pow2_t, j: nat, bi: nat)
+            requires s_loop_inv(a, hcount, j, bi);
+            requires bi < hcount.full
+            ensures |get_full_poly(bi)| == hsize.full;
+            ensures bi + hcount.full < lcount().full;
+            ensures get_even_poly(bi) == even_indexed_items(get_full_poly(bi), hsize);
+            ensures get_odd_poly(bi) == odd_indexed_items(get_full_poly(bi), hsize);
+        {
+            size_count_lemma();
+
+            var ri := bit_rev_int(bi, hcount);
+            var poly := higher[ri];
+
+            level_polys_index_correspondence_lemma(higher, hsize, ri, lower);
+
+            assert even_indexed_items(poly, hsize) == lower[2 * ri];
+            assert odd_indexed_items(poly, hsize) == lower[2 * ri + 1];
+
+            bit_rev_int_lemma0(bi, hcount);
+            bit_rev_int_lemma1(bi, hcount);
+            // assert bit_rev_int(bi, lcount()) == 2 * ri;
+            // assert bit_rev_int(bi + hcount.full, lcount()) == 2 * ri + 1;
+        }
+
+        lemma ct_butterfly_even_lemma(a: n_sized, hcount: pow2_t, j: nat, bi: nat, s: nat, w: elem)
+            requires s_loop_inv(a, hcount, j, bi);
+            requires s == bi + (2*j) * hcount.full;
+            requires bi < hcount.full
+            requires w == mqmul(x_value(2 * j, hcount), R);
+            ensures s + hcount.full < N.full;
+            ensures bi + hcount.full < lcount().full;
+            ensures poly_eval(get_full_poly(bi), x_value(2*j, hcount)) == mqadd(a[s], montmul(a[s+hcount.full], w));
+        {
+            size_count_lemma();
+            lower_points_view_value_lemma(a, hcount, j, bi, s);
+            var e := a[s];
+            var o := a[s+hcount.full];
+            var p := montmul(o, w);
+
+            gbassert IsModEquivalent(p, o * x_value(2 * j, hcount), Q) by {
+                assert IsModEquivalent(p, o * w * R_INV, Q) by {
+                    LemmaSmallMod(p, Q);
+                }
+                assert IsModEquivalent(R_INV * R, 1, Q) by {
+                    Nth_root_lemma();
+                }
+                assert IsModEquivalent(w, x_value(2 * j, hcount) * R, Q) by {
+                    LemmaSmallMod(w, Q);
+                }
+            }
+
+            assert p == (o * x_value(2 * j, hcount)) % Q by {
+                LemmaSmallMod(p, Q);
+            }
+
+            var sum := mqadd(e, p);
+            var diff := mqsub(e, p);
+
+            var e_poly := get_even_poly(bi);
+            var o_poly := get_odd_poly(bi);
+            var f_poly := get_full_poly(bi);
+
+            level_polys_bitrev_index_correspondence_lemma(a, hcount, j, bi);
+
+            var x := x_value(2*j, hcount);
+            var sqr := x_value(j, lcount());
+
+            assert e == poly_eval(e_poly, sqr);
+            assert o == poly_eval(o_poly, sqr);
+
+            x_value_even_square_lemma(j, x);
+
+            poly_eval_split_lemma(f_poly, e_poly, o_poly, hsize, x);
+        }
+
+        lemma ct_butterfly_odd_lemma(a: n_sized, hcount: pow2_t, j: nat, bi: nat, s: nat, w: elem)
+            requires s_loop_inv(a, hcount, j, bi);
+            requires bi < hcount.full
+            requires s == bi + (2*j) * hcount.full;
+            requires w == mqmul(x_value(2 * j, hcount), R);
+            ensures s + hcount.full < N.full;
+            ensures bi + hcount.full < lcount().full;
+            ensures poly_eval(get_full_poly(bi), x_value(2*j+1, hcount))
+                == mqsub(a[s], montmul(a[s+hcount.full], w));
+        {
+            size_count_lemma();
+            lower_points_view_value_lemma(a, hcount, j, bi, s);
+            var e := a[s];
+            var o := a[s+hcount.full];
+            var p := montmul(o, w);
+
+            gbassert IsModEquivalent(p, o * x_value(2*j, hcount), Q) by {
+                assert IsModEquivalent(p, o * w * R_INV, Q) by {
+                    LemmaSmallMod(p, Q);
+                }
+                assert IsModEquivalent(R_INV * R, 1, Q) by {
+                    Nth_root_lemma();
+                }
+                assert IsModEquivalent(w, x_value(2*j, hcount) * R, Q) by {
+                    LemmaSmallMod(w, Q);
+                }
+            }
+
+            assert p == (o * x_value(2 * j, hcount)) % Q by {
+                LemmaSmallMod(p, Q);
+            }
+
+            var diff := mqsub(e, p);
+
+            var e_poly := get_even_poly(bi);
+            var o_poly := get_odd_poly(bi);
+            var f_poly := get_full_poly(bi);
+
+            var x_e := x_value(2*j, hcount);
+            var x_o := x_value(2*j+1, hcount);
+        
+            x_value_odd_square_lemma(j, x_o);
+
+            level_polys_bitrev_index_correspondence_lemma(a, hcount, j, bi);
+
+            var sqr := x_value(j, lcount());
+
+            calc == {
+                x_o;
+                {
+                    LemmaMulNonnegative(bit_rev_int(2*j+1, hsize), hcount.full);
+                }
+                mqpow(OMEGA_INV, bit_rev_int(2*j+1, hsize) * hcount.full);
+                {
+                    bit_rev_int_lemma3(j, lsize());
+                    assert bit_rev_int(2*j+1, hsize) == bit_rev_int(j, lsize()) + lsize().full;
+                }
+                mqpow(OMEGA_INV, (bit_rev_int(j, lsize()) + lsize().full) * hcount.full);
+                {
+                    LemmaMulIsDistributive(hcount.full, bit_rev_int(j, lsize()), lsize().full);
+                }
+                mqpow(OMEGA_INV, bit_rev_int(j, lsize()) * hcount.full + lsize().full * hcount.full);
+                {
+                    bit_rev_int_lemma2(j, lsize());
+                }
+                mqpow(OMEGA_INV, bit_rev_int(2 * j, hsize) * hcount.full + lsize().full * hcount.full);
+                {
+                    LemmaMulNonnegative(bit_rev_int(2 * j, hsize), hcount.full);
+                    inv_half_rotation_lemma(bit_rev_int(2 * j, hsize) * hcount.full);
+                    Nth_root_lemma();
+                    assert lsize().full * hcount.full == N.full / 2;
+                }
+                (Q - x_e) % Q;
+                {
+                    assume x_e != 0;
+                }
+                Q - x_e;
+            }
+
+            calc == {
+                diff;
+                mqsub(e, mqmul(o, x_e));
+                {
+                    LemmaMulNonnegative(o, x_e);
+                }
+                (e as int - ((o * x_e) % Q)) % Q;
+                {
+                    LemmaSubModNoopRight(e, o * x_e, Q);
+                }
+                (e as int - (o * x_e)) % Q;
+                (e as int - ((o * (Q - x_o)))) % Q;
+                {
+                    LemmaMulIsCommutative(o, Q - x_o);
+                }
+                (e as int - (((Q - x_o) * o))) % Q;
+                {
+                    LemmaMulIsDistributive(o, Q, x_o);
+                }
+                (e as int - (Q * o- x_o * o)) % Q;
+                (e as int + x_o * o - Q * o) % Q;
+                {
+                    LemmaModMultiplesVanish(e as int + x_o * o, -(o as int), Q);
+                }
+                (e as int + x_o * o) % Q;
+                {
+                    LemmaAddModNoop(e, x_o * o, Q);
+                }
+                ((e % Q) + (x_o * o) % Q) % Q;
+                {
+                    LemmaSmallMod(e, Q);
+                }
+                (e + (x_o * o) % Q) % Q;
+                (e + mqmul(x_o, o)) % Q;
+                mqadd(e, mqmul(x_o, o));
+                mqadd(poly_eval(e_poly, sqr), mqmul(x_o, poly_eval(o_poly, sqr)));
+                {
+                    poly_eval_split_lemma(f_poly, e_poly, o_poly, hsize, x_o);
+                }
+                poly_eval(f_poly, x_o);
+            }
+        }
+
+        predicate s_loop_update(a: n_sized, a': n_sized, hcount: pow2_t, j: nat, bi: nat)
+            requires s_loop_inv(a, hcount, j, bi);
+            requires bi < hcount.full
+        {
+            var s := bi + (2*j) * hcount.full;
+            var w := mqmul(x_value(2 * j, hcount), R);
+            point_view_index_bound_lemma(bi, 2 * j+1, hsize);
+            point_view_index_bound_lemma(bi, 2 * j, hsize);
+            LemmaMulIsDistributive(hcount.full, 2*j, 1);
+            assert (2*j) * hcount.full + hcount.full == (2*j + 1) * hcount.full;
+            var s' := s+hcount.full; 
+            a' == a[s := mqadd(a[s], montmul(a[s'], w))]
+                [s' := mqsub(a[s], montmul(a[s'], w))]
+        }
+
+        lemma s_loop_perserves_higher_inv_lemma(a: n_sized, a': n_sized, hcount: pow2_t, j: nat, bi: nat)
+            requires s_loop_inv(a, hcount, j, bi);
+            requires bi < hcount.full
+            requires s_loop_update(a, a', hcount, j, bi);
+            ensures s_loop_higher_inv(a', hcount, j, bi+1);
+        {
+            reveal s_loop_higher_inv();
+
+            var s := higher_points_view_index_lemma(a, hcount, j, bi);
+            var s' := s+hcount.full;
+            assert s == point_view_index(bi, 2*j, hsize);
+            assert s' == point_view_index(bi, 2*j + 1, hsize);
+
+            // var vo := mqadd(a[s], mqmul(a[s'], w));
+            // var ve := mqsub(a[s], mqmul(a[s'], w));
+
+            var hpoints := level_points_view(a, hsize);
+            var hpoints' := level_points_view(a', hsize);
+            var size := hsize.full;
+
+            forall i | (0 <= i < bi || bi + 1 <= i < hcount.full)
+                ensures hpoints[i] == hpoints'[i];
+                ensures 0 <= i < bi ==> points_eval_prefix_inv(hpoints'[i], higher[bit_rev_int(i, hcount)], x_value, 2*j+2, hcount);
+                ensures bi + 1 <= i < hcount.full ==> points_eval_prefix_inv(hpoints'[i], higher[bit_rev_int(i, hcount)], x_value, 2*j, hcount);
+            {
+                var left := hpoints[i];
+                var right := hpoints'[i];
+    
+                assert left == right by {
+                    forall k | 0 <= k < hsize.full 
+                        ensures a[point_view_index(i, k, hsize)]
+                            == a'[point_view_index(i, k, hsize)];
+                    {
+                        point_view_index_disjont_lemma(i, k, bi, 2*j, hsize);
+                        point_view_index_disjont_lemma(i, k, bi, 2*j+1, hsize);
+                    }
+                }
+            }
+
+            var left := hpoints[bi];
+            var right := hpoints'[bi];
+            var poly := higher[bit_rev_int(bi, hcount)];
+
+            assert points_eval_prefix_inv(right, poly, x_value, 2*j+2, hcount) by {
+                reveal points_eval_prefix_inv();
+                forall k | 0 <= k < 2*j+2 
+                    ensures poly_eval(poly, x_value(k, hcount)) == right[k];
+                {
+                    if k != 2*j && k != 2*j+1 {
+                        point_view_index_disjont_lemma(bi, k, bi, 2*j, hsize);
+                        point_view_index_disjont_lemma(bi, k, bi, 2*j+1, hsize);
+                        assert right[k] == left[k];
+                    } else {
+                        var w := mqmul(x_value(2 * j, hcount), R);
+                        ct_butterfly_even_lemma(a, hcount, j, bi, s, w);
+                        ct_butterfly_odd_lemma(a, hcount, j, bi, s, w);
+                    }
+                }
+            }
+        }
+
+        lemma s_loop_perserves_lower_inv_lemma(a: n_sized, a': n_sized, hcount: pow2_t, j: nat, bi: nat)
+            requires s_loop_inv(a, hcount, j, bi);
+            requires bi < hcount.full
+            requires s_loop_update(a, a', hcount, j, bi);
+            ensures s_loop_lower_inv(a', hcount, j, bi+1);
+        {
+            size_count_lemma();
+            var s := lower_points_view_index_lemma(a, hcount, j, bi);
+            var s' := s+hcount.full;
+            assert s == point_view_index(bi, j, lsize());
+            assert s+hcount.full == point_view_index(bi+hcount.full, j, lsize());
+
+            reveal s_loop_lower_inv();
+
+            var lpoints := level_points_view(a, lsize());
+            var lpoints' := level_points_view(a', lsize());
+            var lsize := lsize();
+            var count := lcount();
+
+            forall i | (bi + 1 <= i < hcount.full || bi + hcount.full + 1 <= i < count.full) 
+                ensures points_eval_suffix_inv(lpoints'[i], lower[bit_rev_int(i, count)], x_value, j, count);
+            {
+                var left := lpoints[i];
+                var right := lpoints'[i];
+    
+                assert left == right by {
+                    forall k | 0 <= k < lsize.full 
+                        ensures a[point_view_index(i, k, lsize)]
+                            == a'[point_view_index(i, k, lsize)];
+                    {
+                        point_view_index_disjont_lemma(i, k, bi, j, lsize);
+                        point_view_index_disjont_lemma(i, k, bi + hcount.full, j, lsize);
+                    }
+                }
+            }
+        
+            forall i | (0 <= i <= bi || hcount.full <= i <= bi + hcount.full)
+                ensures points_eval_suffix_inv(lpoints'[i], lower[bit_rev_int(i, count)], x_value, j+1, count);
+            {
+                var left := lpoints[i];
+                var right := lpoints'[i];
+                var poly := lower[bit_rev_int(i, count)];
+
+                if i == bi || i == bi + hcount.full {
+                    assert points_eval_suffix_inv(right, poly, x_value, j+1, count) by {
+                        reveal points_eval_suffix_inv();
+                        forall k | j + 1 <= k < lsize.full
+                            ensures right[k] == left[k];
+                            ensures poly_eval(poly, x_value(k, count)) == right[k];
+                        {
+                            // assert left[k] == a[point_view_index(bi, k, lsize)];
+                            // assert right[k] == a'[point_view_index(bi, k, lsize)];
+
+                            point_view_index_disjont_lemma(bi, k, bi, j, lsize);
+                            point_view_index_disjont_lemma(bi, k, bi + hcount.full, j, lsize);
+                            point_view_index_disjont_lemma(bi + hcount.full, k, bi, j, lsize);
+                            point_view_index_disjont_lemma(bi + hcount.full, k, bi + hcount.full, j, lsize);
+
+                            assert right[k] == left[k];
+                        }
+                    }
+                } else {
+                    assert left == right by {
+                        forall k | 0 <= k < lsize.full 
+                            ensures a[point_view_index(i, k, lsize)]
+                                == a'[point_view_index(i, k, lsize)];
+                        {
+                            point_view_index_disjont_lemma(i, k, bi, j, lsize);
+                            point_view_index_disjont_lemma(i, k, bi + hcount.full, j, lsize);
+                        }
+                    }
+                }
+            }
+        }
+
+        lemma s_loop_inv_peri_lemma(a: n_sized, a': n_sized, hcount: pow2_t, j: nat, bi: nat)
+            requires s_loop_inv(a, hcount, j, bi);
+            requires bi < hcount.full
+            requires s_loop_update(a, a', hcount, j, bi);
+            ensures s_loop_inv(a', hcount, j, bi+1);
+        {
+            s_loop_perserves_higher_inv_lemma(a, a', hcount, j, bi);
+            s_loop_perserves_lower_inv_lemma(a, a', hcount, j, bi);
+        }
+
+        lemma s_loop_inv_pre_lemma(a: n_sized, hcount: pow2_t, j: nat)
+            requires j_loop_inv(a, hcount, j);
+            requires j < lsize().full;
+            ensures s_loop_inv(a, hcount, j, 0);
+        {
+            assert s_loop_higher_inv(a, hcount, j, 0) by {
+                reveal s_loop_higher_inv();
+                reveal j_loop_higher_inv();
+            }
+
+            size_count_lemma();
+    
+            assert s_loop_lower_inv(a, hcount, j, 0) by {
+                reveal s_loop_lower_inv();
+                reveal j_loop_lower_inv();
+
+                var lcount := lcount();
+                var lpoints := level_points_view(a, lsize());
+
+                forall i | (0 <= i < hcount.full || hcount.full <= i < lcount.full)
+                    ensures points_eval_suffix_inv(lpoints[i], lower[bit_rev_int(i, lcount)], x_value, j, lcount);
+                {
+                    assert (0 <= i < hcount.full || hcount.full <= i < lcount.full)
+                        ==> (0 <= i < lcount.full);
+                }
+            }
+        }
+
+        lemma s_loop_inv_post_lemma(a: n_sized, hcount: pow2_t, j: nat, bi: nat)
+            requires s_loop_inv(a, hcount, j, bi);
+            requires bi == hcount.full;
+            ensures j_loop_inv(a, hcount, j + 1)
+        {
+            assert j_loop_higher_inv(a, hcount, j+1) by {
+                var hpoints := level_points_view(a, hsize);
+                reveal s_loop_higher_inv();
+                forall i | 0 <= i < |hpoints|
+                    ensures points_eval_prefix_inv(hpoints[i], higher[bit_rev_int(i, hcount)], x_value, 2*j+2, hcount);
+                {
+                }
+                reveal j_loop_higher_inv();
+            }
+
+            size_count_lemma();
+
+            assert j_loop_lower_inv(a, hcount, j+1) by {
+                var lcount := lcount();
+                var lpoints := level_points_view(a, lsize());
+                reveal s_loop_lower_inv();
+                forall i | 0 <= i < |lpoints|
+                    ensures points_eval_suffix_inv(lpoints[i], lower[bit_rev_int(i, lcount)], x_value, j+1, lcount);
+                {
+                }
+                reveal j_loop_lower_inv();
+            }
+        }
+
+        lemma j_loop_inv_pre_lemma(a: n_sized, hcount: pow2_t)
+            requires t_loop_inv(a, hcount);
+            ensures j_loop_inv(a, hcount, 0);
+        {
+            assert j_loop_higher_inv(a, hcount, 0) by {
+                var hpoints := level_points_view(a, hsize);
+                forall i | 0 <= i < hcount.full
+                    ensures points_eval_prefix_inv(hpoints[i], higher[bit_rev_int(i, hcount)], x_value, 0, hcount);
+                {
+                    unifromly_sized_instance_lemma(hpoints, hsize, i);
+                    unifromly_sized_instance_lemma(higher, hsize, bit_rev_int(i, hcount));
+                    points_eval_prefix_inv_vacuous_lemma(hpoints[i], higher[bit_rev_int(i, hcount)], x_value, hcount);
+                }
+                reveal j_loop_higher_inv();
+            }
+    
+            assert j_loop_lower_inv(a, hcount, 0) by {
+                reveal t_loop_low_inv();
+                var lcount := lcount();
+                var lpoints := level_points_view(a, lsize());
+                forall i | 0 <= i < lcount.full
+                    ensures points_eval_suffix_inv(lpoints[i], lower[bit_rev_int(i, lcount)], x_value, 0, lcount)
+                {
+                    reveal points_eval_suffix_inv();
+                }
+                reveal j_loop_lower_inv();
+            }
+        }
+
+        function next_t_loop_view(hcount: pow2_t): (v': intt_loop_view)
+            requires loop_view_wf();
+            requires 0 <= hsize.exp <= N.exp;
+            requires 0 <= hcount.exp < N.exp;
+            requires hsize == block_size(hcount);
+            ensures v'.loop_view_wf();
+        {
+            if hsize.exp == N.exp then
+                this
+            else
+                var v' := intt_loop_view(higher, build_higher_level(higher, hsize), pow2_double(hsize));
+                build_higher_inverse_lemma(higher, hsize);
+                v'
+        }
+
+        lemma j_loop_inv_post_lemma(a: n_sized, hcount: pow2_t, j: nat)
+            returns (v': intt_loop_view)
+            requires j_loop_inv(a, hcount, j);
+            requires j == lsize().full;
+            requires 0 <= hsize.exp <= N.exp;
+            ensures v' == next_t_loop_view(hcount);
+            ensures hsize.exp < N.exp ==> v'.t_loop_inv(a, pow2_half(hcount));
+            ensures hsize.exp == N.exp ==> v'.t_loop_end(a);
+        {
+            reveal j_loop_higher_inv();
+            size_count_lemma();
+            var hpoints := level_points_view(a, hsize);
+
+            forall i | 0 <= i < hcount.full
+                ensures points_eval_inv(hpoints[i], higher[bit_rev_int(i, hcount)], x_value, hcount);
+            {
+                reveal points_eval_suffix_inv();
+                reveal points_eval_prefix_inv();
+            }
+
+            v' := next_t_loop_view(hcount);
+            v'.size_count_lemma();
+
+            if hsize.exp < N.exp {
+                assert v'.t_loop_inv(a, pow2_half(hcount)) by {
+                    reveal v'.t_loop_low_inv();
+                    assert v'.t_loop_low_inv(a, v'.hcount());
+                }
+            } else {
+                Nth_root_lemma();
+                assert hsize.exp == N.exp;
+                assert hsize.full == N.full;
+                assert |hpoints| * N.full == N.full;
+                LemmaFundamentalDivModConverse(|hpoints| * N.full, N.full, 1, 0);
+                assert |hpoints| == 1;
+                assert bit_rev_int(0, hcount) == 0;
+            }
+        }
+    }
+}
